Probably bug with interface.

src/riot/x509/X509.ExtFields.KeyUsage.fst
@@ -29,37 +29,21 @@ open FStar.Integers
  * #define MBEDTLS_X509_KU_DECIPHER_ONLY              (0x8000)  /* bit 8 */
  *)
 
-let valid_key_usage
-  (i: int_32)
-: Type0
-= 0l < i /\ (* at least one usage *)
-  (i <= 0xFFl \/ i / 0x100l == 0x80l)
-
-let key_usage_payload_t = i: int_32
-                     { valid_key_usage i }
-
-let x509_KU_DIGITAL_SIGNATURE :key_usage_payload_t = 0x80l    (* bit 0 *)
-let x509_KU_NON_REPUDIATION   :key_usage_payload_t = 0x40l    (* bit 1 *)
-let x509_KU_KEY_ENCIPHERMENT  :key_usage_payload_t = 0x20l    (* bit 2 *)
-let x509_KU_DATA_ENCIPHERMENT :key_usage_payload_t = 0x10l    (* bit 3 *)
-let x509_KU_KEY_AGREEMENT     :key_usage_payload_t = 0x08l    (* bit 4 *)
-let x509_KU_KEY_CERT_SIGN     :key_usage_payload_t = 0x04l    (* bit 5 *)
-let x509_KU_CRL_SIGN          :key_usage_payload_t = 0x02l    (* bit 6 *)
-let x509_KU_ENCIPHER_ONLY     :key_usage_payload_t = 0x01l    (* bit 7 *)
-let x509_KU_DECIPHER_ONLY     :key_usage_payload_t = 0x8000l  (* bit 8 *)
+let x509_KU_DIGITAL_SIGNATURE = 0x80l    (* bit 0 *)
+let x509_KU_NON_REPUDIATION   = 0x40l    (* bit 1 *)
+let x509_KU_KEY_ENCIPHERMENT  = 0x20l    (* bit 2 *)
+let x509_KU_DATA_ENCIPHERMENT = 0x10l    (* bit 3 *)
+let x509_KU_KEY_AGREEMENT     = 0x08l    (* bit 4 *)
+let x509_KU_KEY_CERT_SIGN     = 0x04l    (* bit 5 *)
+let x509_KU_CRL_SIGN          = 0x02l    (* bit 6 *)
+let x509_KU_ENCIPHER_ONLY     = 0x01l    (* bit 7 *)
+let x509_KU_DECIPHER_ONLY     = 0x8000l  (* bit 8 *)
 
 (* FIXME: Can we normalize bitwise operators? *)
-let lemma_key_usage_close_under_or
-  (ku1 ku2: key_usage_payload_t)
-: Lemma (
-  valid_key_usage (ku1 |^ ku2)
-)
+let lemma_key_usage_close_under_or ku1 ku2
 = admit()
 
-let op_ku_with
-  (ku1 ku2: key_usage_payload_t)
-: Tot (ku: key_usage_payload_t
-           { ku == (ku1 |^ ku2) })
+let op_ku_with ku1 ku2
 = [@inline_let]let ku: int_32 = ku1 |^ ku2 in
   lemma_key_usage_close_under_or ku1 ku2;
   ku
@@ -112,7 +96,8 @@ let lemma_synth_x509_key_usage_injective ()
 let _synth_x509_key_usage_payload_inverse
   (ku: key_usage_payload_t)
 : GTot (bs: parse_filter_refine _filter_x509_key_usage_payload
-            { _synth_x509_key_usage_payload bs == ku })
+            { _synth_x509_key_usage_payload bs == ku /\
+              length_of_asn1_primitive_TLV #BIT_STRING bs == 5 })
 = let b0: byte = FStar.Int.Cast.int32_to_uint8 (ku % 0x100l) in
   let b1: byte = FStar.Int.Cast.int32_to_uint8 (ku / 0x100l) in
   let s = Seq.createL [b0; b1] in
@@ -123,7 +108,6 @@ let _synth_x509_key_usage_payload_inverse
 #pop-options
 
 let _parse_x509_key_usage_payload
-: parser _ key_usage_payload_t
 = lemma_synth_x509_key_usage_injective ();
   parse_asn1_TLV_of_type BIT_STRING
   `parse_filter`
@@ -132,7 +116,6 @@ let _parse_x509_key_usage_payload
   _synth_x509_key_usage_payload
 
 let _serialize_x509_key_usage_payload
-: serializer _parse_x509_key_usage_payload
 = serialize_synth
   (* p1 *) (parse_asn1_TLV_of_type BIT_STRING
             `parse_filter`
@@ -144,6 +127,7 @@ let _serialize_x509_key_usage_payload
   (* g1 *) (_synth_x509_key_usage_payload_inverse)
   (* Prf*) (lemma_synth_x509_key_usage_injective ())
 
+// NOTE: This is not exposed yet.
 let lemma_serialize_x509_key_usage_payload_unfold
   (ku: key_usage_payload_t)
 : Lemma (
@@ -162,13 +146,17 @@ let lemma_serialize_x509_key_usage_payload_unfold
   (* Prf*) (lemma_synth_x509_key_usage_injective ())
   (* in *) (ku)
 
-let lemma_serialize_x509_key_usage_payload_size
+let lemma_serialize_x509_key_usage_payload_size_aux
   (ku: key_usage_payload_t)
 : Lemma (
   length_of_opaque_serialization _serialize_x509_key_usage_payload ku ==
-  length_of_asn1_primitive_TLV #BIT_STRING (_synth_x509_key_usage_payload_inverse ku)
+  length_of_asn1_primitive_TLV #BIT_STRING (_synth_x509_key_usage_payload_inverse ku) /\
+  length_of_asn1_primitive_TLV #BIT_STRING (_synth_x509_key_usage_payload_inverse ku) == 5
 )
 = lemma_serialize_x509_key_usage_payload_unfold ku
+
+let lemma_serialize_x509_key_usage_payload_size ku
+= lemma_serialize_x509_key_usage_payload_size_aux ku
 
 (* Complete X509 Key Usage Parser and Serializer for
  *
@@ -181,46 +169,7 @@ let lemma_serialize_x509_key_usage_payload_size
  *
  *)
 
-let key_usage_t
-= inbound_sequence_value_of
-    (OID_KEY_USAGE
-     `serialize_envelop_OID_with`
-    (OCTET_STRING
-     `serialize_asn1_envelop_tag_with_TLV`
-     _serialize_x509_key_usage_payload))
-
-let parse_x509_key_usage
-: parser (parse_asn1_envelop_tag_with_TLV_kind SEQUENCE) key_usage_t
-= key_usage_t
-  `coerce_parser`
- (parse_asn1_sequence_TLV
-    (OID_KEY_USAGE
-     `serialize_envelop_OID_with`
-    (OCTET_STRING
-     `serialize_asn1_envelop_tag_with_TLV`
-     _serialize_x509_key_usage_payload)))
-
-let serialize_x509_key_usage
-: serializer (parse_x509_key_usage)
-= coerce_parser_serializer
-  (* p *) (parse_x509_key_usage)
-  (* s *) (serialize_asn1_sequence_TLV
-            (OID_KEY_USAGE
-             `serialize_envelop_OID_with`
-            (OCTET_STRING
-             `serialize_asn1_envelop_tag_with_TLV`
-             _serialize_x509_key_usage_payload)))
-  (*prf*) ()
-
-let lemma_serialize_x509_key_usage_unfold
-  (x: key_usage_t)
-: Lemma ( predicate_serialize_asn1_sequence_TLV_unfold
-            (OID_KEY_USAGE
-             `serialize_envelop_OID_with`
-            (OCTET_STRING
-             `serialize_asn1_envelop_tag_with_TLV`
-             _serialize_x509_key_usage_payload))
-            x )
+let lemma_serialize_x509_key_usage_unfold x
 = lemma_serialize_asn1_sequence_TLV_unfold
     (OID_KEY_USAGE
      `serialize_envelop_OID_with`
@@ -229,15 +178,7 @@ let lemma_serialize_x509_key_usage_unfold
              _serialize_x509_key_usage_payload))
     x
 
-let lemma_serialize_x509_key_usage_size
-  (x: key_usage_t)
-: Lemma ( predicate_serialize_asn1_sequence_TLV_size
-            (OID_KEY_USAGE
-             `serialize_envelop_OID_with`
-            (OCTET_STRING
-             `serialize_asn1_envelop_tag_with_TLV`
-             _serialize_x509_key_usage_payload))
-            x )
+let lemma_serialize_x509_key_usage_size x
 = lemma_serialize_asn1_sequence_TLV_size
     (OID_KEY_USAGE
      `serialize_envelop_OID_with`
@@ -246,24 +187,11 @@ let lemma_serialize_x509_key_usage_size
              _serialize_x509_key_usage_payload))
     x
 
-#restart-solver
-#push-options "--z3rlimit 64 --fuel 0 --fuel 0"
-let length_of_x509_key_usage
-  (ku: key_usage_payload_t)
-: GTot (asn1_TLV_length_of_type SEQUENCE)
-= length_of_TLV
-    SEQUENCE
-    ( length_of_asn1_primitive_TLV #BIT_STRING (_synth_x509_key_usage_payload_inverse ku) +
-      ( length_of_TLV
-          OCTET_STRING
-          ( length_of_asn1_primitive_TLV #OID OID_KEY_USAGE ) ) )
+(* Stuck here *)
+let () = ()
 
-let lemma_serialize_x509_key_usage_size_exact
-  (x: key_usage_t)
-: Lemma (
-  length_of_opaque_serialization serialize_x509_key_usage x
-  == length_of_x509_key_usage (snd x)
-)
+#push-options "--z3rlimit 64 --fuel 0 --fuel 0"
+let lemma_serialize_x509_key_usage_size_exact x
 = lemma_serialize_x509_key_usage_size x;
   (**) lemma_serialize_envelop_OID_with_size
          (fst x)
@@ -276,7 +204,8 @@ let lemma_serialize_x509_key_usage_size_exact
               (OCTET_STRING)
               (_serialize_x509_key_usage_payload)
               (snd x);
-            (**) lemma_serialize_x509_key_usage_payload_size (snd x)
+            (**) lemma_serialize_x509_key_usage_payload_size (snd x);
+            (**) lemma_serialize_x509_key_usage_payload_size_aux (snd x)
 #pop-options
 
 open ASN1.Low
