src/riot/x509/X509.ExtFields.KeyUsage.fsti
@@ -1,0 +1,223 @@
+module X509.ExtFields.KeyUsage
+
+open LowParse.Spec.Base
+open LowParse.Spec.Combinators
+
+open ASN1.Base
+open ASN1.Spec
+open ASN1.Low
+
+open X509.Base
+
+module B32 = FStar.Bytes
+
+open FStar.Integers
+
+(*
+ * /*
+ *  * X.509 v3 Key Usage Extension flags
+ *  * Reminder: update x509_info_key_usage() when adding new flags.
+ *  */
+ * #define MBEDTLS_X509_KU_DIGITAL_SIGNATURE            (0x80)  /* bit 0 */
+ * #define MBEDTLS_X509_KU_NON_REPUDIATION              (0x40)  /* bit 1 */
+ * #define MBEDTLS_X509_KU_KEY_ENCIPHERMENT             (0x20)  /* bit 2 */
+ * #define MBEDTLS_X509_KU_DATA_ENCIPHERMENT            (0x10)  /* bit 3 */
+ * #define MBEDTLS_X509_KU_KEY_AGREEMENT                (0x08)  /* bit 4 */
+ * #define MBEDTLS_X509_KU_KEY_CERT_SIGN                (0x04)  /* bit 5 */
+ * #define MBEDTLS_X509_KU_CRL_SIGN                     (0x02)  /* bit 6 */
+ * #define MBEDTLS_X509_KU_ENCIPHER_ONLY                (0x01)  /* bit 7 */
+ * #define MBEDTLS_X509_KU_DECIPHER_ONLY              (0x8000)  /* bit 8 */
+ *)
+
+let valid_key_usage
+  (i: int_32)
+: Type0
+= 0l < i /\ (* at least one usage *)
+  (i <= 0xFFl \/ i / 0x100l == 0x80l)
+
+let key_usage_payload_t = i: int_32
+                     { valid_key_usage i }
+
+val x509_KU_DIGITAL_SIGNATURE :key_usage_payload_t // = 0x80l    (* bit 0 *)
+val x509_KU_NON_REPUDIATION   :key_usage_payload_t // = 0x40l    (* bit 1 *)
+val x509_KU_KEY_ENCIPHERMENT  :key_usage_payload_t // = 0x20l    (* bit 2 *)
+val x509_KU_DATA_ENCIPHERMENT :key_usage_payload_t // = 0x10l    (* bit 3 *)
+val x509_KU_KEY_AGREEMENT     :key_usage_payload_t // = 0x08l    (* bit 4 *)
+val x509_KU_KEY_CERT_SIGN     :key_usage_payload_t // = 0x04l    (* bit 5 *)
+val x509_KU_CRL_SIGN          :key_usage_payload_t // = 0x02l    (* bit 6 *)
+val x509_KU_ENCIPHER_ONLY     :key_usage_payload_t // = 0x01l    (* bit 7 *)
+val x509_KU_DECIPHER_ONLY     :key_usage_payload_t // = 0x8000l  (* bit 8 *)
+
+val lemma_key_usage_close_under_or
+  (ku1 ku2: key_usage_payload_t)
+: Lemma (
+  valid_key_usage (ku1 |^ ku2)
+)
+
+val op_ku_with
+  (ku1 ku2: key_usage_payload_t)
+: Tot (ku: key_usage_payload_t
+           { ku == (ku1 |^ ku2) })
+
+let _parse_x509_key_usage_payload_kind
+: parser_kind
+= parse_filter_kind (parse_asn1_TLV_kind_of_type BIT_STRING)
+
+val _parse_x509_key_usage_payload
+: parser _parse_x509_key_usage_payload_kind key_usage_payload_t
+
+val _serialize_x509_key_usage_payload
+: serializer _parse_x509_key_usage_payload
+
+// NOTE: Drop the support for reasoning about actual byte content for now
+// val lemma_serialize_x509_key_usage_payload_unfold
+//   (ku: key_usage_payload_t)
+// : Lemma (
+//   serialize _serialize_x509_key_usage_payload ku ==
+//   serialize (serialize_asn1_TLV_of_type BIT_STRING) (_synth_x509_key_usage_payload_inverse ku)
+// )
+
+let length_of_x509_key_usage_payload ()
+: GTot (nat)
+= 5
+
+let len_of_x509_key_usage_payload ()
+: Tot (len: asn1_value_int32_of_type SEQUENCE
+            { v len == length_of_x509_key_usage_payload () })
+= 5ul
+
+val lemma_serialize_x509_key_usage_payload_size
+  (ku: key_usage_payload_t)
+: Lemma (
+  length_of_opaque_serialization _serialize_x509_key_usage_payload ku ==
+  length_of_x509_key_usage_payload ()
+)
+
+(* Complete X509 Key Usage Parser and Serializer for
+ *
+ *  SEQUENCE {
+ *    extID   : OID
+ *    extValue: OCTET_STRING {
+ *      key_usage    : key_usage_payload_t
+ *    }
+ *  }
+ *
+ *)
+
+let key_usage_t
+= inbound_sequence_value_of
+    (OID_KEY_USAGE
+     `serialize_envelop_OID_with`
+    (OCTET_STRING
+     `serialize_asn1_envelop_tag_with_TLV`
+     _serialize_x509_key_usage_payload))
+
+let parse_x509_key_usage
+: parser (parse_asn1_envelop_tag_with_TLV_kind SEQUENCE) key_usage_t
+= key_usage_t
+  `coerce_parser`
+ (parse_asn1_sequence_TLV
+    (OID_KEY_USAGE
+     `serialize_envelop_OID_with`
+    (OCTET_STRING
+     `serialize_asn1_envelop_tag_with_TLV`
+     _serialize_x509_key_usage_payload)))
+
+let serialize_x509_key_usage
+: serializer (parse_x509_key_usage)
+= coerce_parser_serializer
+  (* p *) (parse_x509_key_usage)
+  (* s *) (serialize_asn1_sequence_TLV
+            (OID_KEY_USAGE
+             `serialize_envelop_OID_with`
+            (OCTET_STRING
+             `serialize_asn1_envelop_tag_with_TLV`
+             _serialize_x509_key_usage_payload)))
+  (*prf*) ()
+
+val lemma_serialize_x509_key_usage_unfold
+  (x: key_usage_t)
+: Lemma ( predicate_serialize_asn1_sequence_TLV_unfold
+            (OID_KEY_USAGE
+             `serialize_envelop_OID_with`
+            (OCTET_STRING
+             `serialize_asn1_envelop_tag_with_TLV`
+             _serialize_x509_key_usage_payload))
+            x )
+
+val lemma_serialize_x509_key_usage_size
+  (x: key_usage_t)
+: Lemma ( predicate_serialize_asn1_sequence_TLV_size
+            (OID_KEY_USAGE
+             `serialize_envelop_OID_with`
+            (OCTET_STRING
+             `serialize_asn1_envelop_tag_with_TLV`
+             _serialize_x509_key_usage_payload))
+            x )
+
+let length_of_x509_key_usage
+  (ku: key_usage_payload_t)
+: GTot (asn1_TLV_length_of_type SEQUENCE)
+= length_of_TLV
+    SEQUENCE
+    ( length_of_x509_key_usage_payload () +
+      ( length_of_TLV
+          OCTET_STRING
+          ( length_of_asn1_primitive_TLV #OID OID_KEY_USAGE ) ) )
+
+val lemma_serialize_x509_key_usage_size_exact
+  (x: key_usage_t)
+: Lemma (
+  length_of_opaque_serialization serialize_x509_key_usage x
+  == length_of_x509_key_usage (snd x)
+)
+
+open ASN1.Low
+
+let len_of_x509_key_usage
+  (ku: key_usage_payload_t)
+: Tot (len: asn1_TLV_int32_of_type SEQUENCE
+            { v len == length_of_x509_key_usage ku })
+= len_of_TLV
+    SEQUENCE
+    ( len_of_x509_key_usage_payload () +
+      ( len_of_TLV
+          OCTET_STRING
+          ( len_of_asn1_primitive_TLV #OID OID_KEY_USAGE ) ) )
+
+val _serialize32_x509_key_usage_payload_backwards
+: serializer32_backwards (_serialize_x509_key_usage_payload)
+
+#set-options "--print_implicits"
+val serialize32_x509_key_usage_backwards
+: serializer32_backwards (serialize_x509_key_usage)
+
+///
+///
+/// Helper constructor
+let x509_get_key_usage
+  (ku: key_usage_payload_t)
+: Tot (key_usage_t)
+=
+  (* Prf *) lemma_serialize_x509_key_usage_payload_size ku;
+  let x: OID_KEY_USAGE
+         `envelop_OID_with_t`
+        (OCTET_STRING
+         `inbound_envelop_tag_with_value_of`
+         _serialize_x509_key_usage_payload)
+    = ( OID_KEY_USAGE, ku ) in
+
+  (* Prf *) lemma_serialize_envelop_OID_with_size
+              (fst x)
+              (OCTET_STRING
+               `serialize_asn1_envelop_tag_with_TLV`
+               _serialize_x509_key_usage_payload)
+              (x);
+  (* Prf *) (**) lemma_serialize_asn1_oid_TLV_of_size (fst x) (fst x);
+  (* Prf *) (**) lemma_serialize_asn1_envelop_tag_with_TLV_size
+                   (OCTET_STRING)
+                   (_serialize_x509_key_usage_payload)
+                   (snd x);
+  (* Prf *)      (**) lemma_serialize_x509_key_usage_payload_size (snd x);
+
+(*return*) x <: key_usage_t
